added signed 8-bit to 64-bit integers

lib/Lib.IntTypes.fst
@@ -27,6 +27,11 @@ let uintv_extensionality #t #l a b =
   | U32  -> UInt32.v_inj a b
   | U64  -> UInt64.v_inj a b
   | U128 -> UInt128.v_inj a b
+  | S8   -> Int8.v_inj a b
+  | S16  -> Int16.v_inj a b
+  | S32  -> Int32.v_inj a b
+  | S64  -> Int64.v_inj a b
+  //| S128 -> Int128.v_inj a b
 
 (* Declared in .fsti: uint8, uint16, uint32, uint64, uint128 *)
 
@@ -40,7 +45,12 @@ let uint #t #l x =
   | U32 -> UInt32.uint_to_t x
   | U64 -> UInt64.uint_to_t x
   | U128 -> UInt128.uint_to_t x
-
+  | S8 -> Int8.int_to_t x
+  | S16 -> Int16.int_to_t x
+  | S32 -> Int32.int_to_t x
+  | S64 -> Int64.int_to_t x
+  //| S128 -> Int128.int_to_t x
+  
 let uintv_injective #t #l a =
   uintv_extensionality a (uint (uint_v a))
 
@@ -60,6 +70,8 @@ let size_to_uint64 x = FStar.Int.Cast.uint32_to_uint64 x
 
 let byte_to_uint8 x = x
 
+let byte_to_int8 x = FStar.Int.Cast.uint8_to_int8 x
+
 let nat_to_uint #t #l x =
   match t with
   | U1 -> u8 x
@@ -68,6 +80,12 @@ let nat_to_uint #t #l x =
   | U32 -> u32 x
   | U64 -> u64 x
   | U128 -> UInt128.uint_to_t x
+  | S8 -> i8 x
+  | S16 -> i16 x
+  | S32 -> i32 x
+  | S64 -> i64 x
+  
+#reset-options "--z3rlimit 500"
 
 let cast #t #l t' l' u  =
   match t, t' with
@@ -77,30 +95,50 @@ let cast #t #l t' l' u  =
   | U1, U32 -> FStar.Int.Cast.uint8_to_uint32 u
   | U1, U64 -> FStar.Int.Cast.uint8_to_uint64 u
   | U1, U128 -> FStar.UInt128.uint64_to_uint128 (FStar.Int.Cast.uint8_to_uint64 u)
+  | U1, S8 -> FStar.Int.Cast.uint8_to_int8 u
+  | U1, S16 -> FStar.Int.Cast.uint8_to_int16 u
+  | U1, S32 -> FStar.Int.Cast.uint8_to_int32 u
+  | U1, S64 -> FStar.Int.Cast.uint8_to_int64 u
   | U8, U1 -> FStar.UInt8.rem u 2uy
   | U8, U8 -> u
   | U8, U16 -> FStar.Int.Cast.uint8_to_uint16 u
   | U8, U32 -> FStar.Int.Cast.uint8_to_uint32 u
   | U8, U64 -> FStar.Int.Cast.uint8_to_uint64 u
   | U8, U128 -> FStar.UInt128.uint64_to_uint128 (FStar.Int.Cast.uint8_to_uint64 u)
+  | U8, S8 -> FStar.Int.Cast.uint8_to_int8 u
+  | U8, S16 -> FStar.Int.Cast.uint8_to_int16 u
+  | U8, S32 -> FStar.Int.Cast.uint8_to_int32 u
+  | U8, S64 -> FStar.Int.Cast.uint8_to_int64 u
   | U16, U1 -> FStar.Int.Cast.uint16_to_uint8 (FStar.UInt16.rem u 2us)
   | U16, U8 -> FStar.Int.Cast.uint16_to_uint8 u
   | U16, U16 -> u
   | U16, U32 -> FStar.Int.Cast.uint16_to_uint32 u
   | U16, U64 -> FStar.Int.Cast.uint16_to_uint64 u
   | U16, U128 -> FStar.UInt128.uint64_to_uint128 (FStar.Int.Cast.uint16_to_uint64 u)
+  | U16, S8 -> FStar.Int.Cast.uint16_to_int8 u
+  | U16, S16 -> FStar.Int.Cast.uint16_to_int16 u
+  | U16, S32 -> FStar.Int.Cast.uint16_to_int32 u
+  | U16, S64 -> FStar.Int.Cast.uint16_to_int64 u
   | U32, U1 -> FStar.Int.Cast.uint32_to_uint8 (FStar.UInt32.rem u 2ul)
   | U32, U8 -> FStar.Int.Cast.uint32_to_uint8 u
   | U32, U16 -> FStar.Int.Cast.uint32_to_uint16 u
   | U32, U32 -> u
   | U32, U64 -> FStar.Int.Cast.uint32_to_uint64 u
   | U32, U128 -> FStar.UInt128.uint64_to_uint128 (FStar.Int.Cast.uint32_to_uint64 u)
+  | U32, S8 -> FStar.Int.Cast.uint32_to_int8 u
+  | U32, S16 -> FStar.Int.Cast.uint32_to_int16 u
+  | U32, S32 -> FStar.Int.Cast.uint32_to_int32 u
+  | U32, S64 -> FStar.Int.Cast.uint32_to_int64 u
   | U64, U1 -> FStar.Int.Cast.uint64_to_uint8 (FStar.UInt64.rem u 2uL)
   | U64, U8 -> FStar.Int.Cast.uint64_to_uint8 u
   | U64, U16 -> FStar.Int.Cast.uint64_to_uint16 u
   | U64, U32 -> FStar.Int.Cast.uint64_to_uint32 u
   | U64, U64 -> u
   | U64, U128 -> FStar.UInt128.uint64_to_uint128 u
+  | U64, S8 -> FStar.Int.Cast.uint64_to_int8 u
+  | U64, S16 -> FStar.Int.Cast.uint64_to_int16 u
+  | U64, S32 -> FStar.Int.Cast.uint64_to_int32 u
+  | U64, S64 -> FStar.Int.Cast.uint64_to_int64 u
   | U128, U1 ->
     assert_norm (pow2 64 * pow2 64 = pow2 128);
     assert_norm (pow2 8 * pow2 56 = pow2 64);
@@ -131,6 +169,65 @@ let cast #t #l t' l' u  =
     FStar.Math.Lemmas.modulo_modulo_lemma (uint_v u) (pow2 64) (pow2 64);
     FStar.UInt128.uint128_to_uint64 u
   | U128, U128 -> u
+  | U128, S8 ->
+    assert_norm (pow2 64 * pow2 64 = pow2 128);
+    assert_norm (pow2 8 * pow2 56 = pow2 64);
+    FStar.Math.Lemmas.modulo_modulo_lemma (uint_v u) (pow2 64) (pow2 64);
+    FStar.Math.Lemmas.modulo_modulo_lemma (uint_v u) (pow2 8) (pow2 56);
+    FStar.Int.Cast.uint64_to_int8 (FStar.UInt128.uint128_to_uint64 u)
+  | U128, S16 ->
+    assert_norm (pow2 64 * pow2 64 = pow2 128);
+    assert_norm (pow2 16 * pow2 48 = pow2 64);
+    FStar.Math.Lemmas.modulo_modulo_lemma (uint_v u) (pow2 64) (pow2 64);
+    FStar.Math.Lemmas.modulo_modulo_lemma (uint_v u) (pow2 16) (pow2 48);
+    FStar.Int.Cast.uint64_to_int16 (FStar.UInt128.uint128_to_uint64 u)
+  | U128, S32 ->
+    assert_norm (pow2 64 * pow2 64 = pow2 128);
+    assert_norm (pow2 32 * pow2 32 = pow2 64);
+    FStar.Math.Lemmas.modulo_modulo_lemma (uint_v u) (pow2 64) (pow2 64);
+    FStar.Math.Lemmas.modulo_modulo_lemma (uint_v u) (pow2 32) (pow2 32);
+    FStar.Int.Cast.uint64_to_int32 (FStar.UInt128.uint128_to_uint64 u)
+  | U128, S64 ->
+    assert_norm (pow2 64 * pow2 64 = pow2 128);
+    FStar.Math.Lemmas.modulo_modulo_lemma (uint_v u) (pow2 64) (pow2 64);
+    FStar.Int.Cast.uint64_to_int64 (FStar.UInt128.uint128_to_uint64 u)  
+  | S8, U1 -> FStar.UInt8.rem (FStar.Int.Cast.int8_to_uint8 u) 2uy
+  | S8, U8 -> FStar.Int.Cast.int8_to_uint8 u
+  | S8, U16 -> FStar.Int.Cast.int8_to_uint16 u
+  | S8, U32 -> FStar.Int.Cast.int8_to_uint32 u
+  | S8, U64 -> FStar.Int.Cast.int8_to_uint64 u
+  | S8, S8 -> u
+  | S8, S16 -> FStar.Int.Cast.int8_to_int16 u
+  | S8, S32 -> FStar.Int.Cast.int8_to_int32 u
+  | S8, S64 -> FStar.Int.Cast.int8_to_int64 u
+  | S16, U1 -> FStar.UInt8.rem (FStar.Int.Cast.int16_to_uint8 u) 2uy
+  | S16, U8 -> FStar.Int.Cast.int16_to_uint8 u
+  | S16, U16 -> FStar.Int.Cast.int16_to_uint16 u
+  | S16, U32 -> FStar.Int.Cast.int16_to_uint32 u
+  | S16, U64 -> FStar.Int.Cast.int16_to_uint64 u
+  | S16, S8 -> FStar.Int.Cast.int16_to_int8 u
+  | S16, S16 -> u
+  | S16, S32 -> FStar.Int.Cast.int16_to_int32 u
+  | S16, S64 -> FStar.Int.Cast.int16_to_int64 u
+  | S32, U1 -> FStar.UInt8.rem (FStar.Int.Cast.int32_to_uint8 u) 2uy
+  | S32, U8 -> FStar.Int.Cast.int32_to_uint8 u
+  | S32, U16 -> FStar.Int.Cast.int32_to_uint16 u
+  | S32, U32 -> FStar.Int.Cast.int32_to_uint32 u
+  | S32, U64 -> FStar.Int.Cast.int32_to_uint64 u
+  | S32, S8 -> FStar.Int.Cast.int32_to_int8 u
+  | S32, S16 -> FStar.Int.Cast.int32_to_int16 u
+  | S32, S32 -> u
+  | S32, S64 -> FStar.Int.Cast.int32_to_int64 u
+  | S64, U1 -> FStar.UInt8.rem (FStar.Int.Cast.int64_to_uint8 u) 2uy
+  | S64, U8 -> FStar.Int.Cast.int64_to_uint8 u
+  | S64, U16 -> FStar.Int.Cast.int64_to_uint16 u
+  | S64, U32 -> FStar.Int.Cast.int64_to_uint32 u
+  | S64, U64 -> FStar.Int.Cast.int64_to_uint64 u
+  | S64, S8 -> FStar.Int.Cast.int64_to_int8 u
+  | S64, S16 -> FStar.Int.Cast.int64_to_int16 u
+  | S64, S32 -> FStar.Int.Cast.int64_to_int32 u
+  | S64, S64 -> u
+  
 
 let add_mod #t #l a b =
   match t with
@@ -140,6 +237,11 @@ let add_mod #t #l a b =
   | U32  -> UInt32.add_mod a b
   | U64  -> UInt64.add_mod a b
   | U128 -> UInt128.add_mod a b
+  | S8 -> Int8.int_to_t (Int.add_mod (Int8.v a) (Int8.v b))
+  | S16 -> Int16.int_to_t (Int.add_mod (Int16.v a) (Int16.v b))
+  | S32 -> Int32.int_to_t (Int.add_mod (Int32.v a) (Int32.v b))
+  | S64 -> Int64.int_to_t (Int.add_mod (Int64.v a) (Int64.v b))
+  
 
 let add_mod_lemma #t #l a b = ()
 
@@ -151,7 +253,11 @@ let add #t #l a b =
   | U32  -> UInt32.add a b
   | U64  -> UInt64.add a b
   | U128 -> UInt128.add a b
-
+  | S8 -> Int8.add a b
+  | S16 -> Int16.add a b
+  | S32 -> Int32.add a b
+  | S64 -> Int64.add a b
+  
 let add_lemma #t #l a b = ()
 
 let incr #t #l a =
@@ -162,7 +268,11 @@ let incr #t #l a =
   | U32  -> UInt32.add a 0x1ul
   | U64  -> UInt64.add a 0x1uL
   | U128 -> UInt128.add a (UInt128.uint_to_t 1)
-
+  | S8 -> Int8.add a 0x1y
+  | S16 -> Int16.add a 0x1s
+  | S32 -> Int32.add a 0x1l
+  | S64 -> Int64.add a 0x1L
+  
 let incr_lemma #t #l a = ()
 
 let mul_mod #t #l a b =
@@ -172,7 +282,11 @@ let mul_mod #t #l a b =
   | U16 -> UInt16.mul_mod a b
   | U32 -> UInt32.mul_mod a b
   | U64 -> UInt64.mul_mod a b
-
+  | S8 -> Int8.int_to_t (Int.mul_mod (Int8.v a) (Int8.v b))
+  | S16 -> Int16.int_to_t (Int.mul_mod (Int16.v a) (Int16.v b))
+  | S32 -> Int32.int_to_t (Int.mul_mod (Int32.v a) (Int32.v b))
+  | S64 -> Int64.int_to_t (Int.mul_mod (Int64.v a) (Int64.v b))
+  
 let mul_mod_lemma #t #l a b = ()
 
 let mul #t #l a b =
@@ -182,7 +296,11 @@ let mul #t #l a b =
   | U16 -> UInt16.mul a b
   | U32 -> UInt32.mul a b
   | U64 -> UInt64.mul a b
-
+  | S8 -> Int8.mul a b
+  | S16 -> Int16.mul a b
+  | S32 -> Int32.mul a b
+  | S64 -> Int64.mul a b
+  
 let mul_lemma #t #l a b = ()
 
 let mul64_wide a b = UInt128.mul_wide a b
@@ -197,6 +315,10 @@ let sub_mod #t #l a b =
   | U32  -> UInt32.sub_mod a b
   | U64  -> UInt64.sub_mod a b
   | U128 -> UInt128.sub_mod a b
+  | S8 -> Int8.int_to_t (Int.sub_mod (Int8.v a) (Int8.v b))
+  | S16 -> Int16.int_to_t (Int.sub_mod (Int16.v a) (Int16.v b))
+  | S32 -> Int32.int_to_t (Int.sub_mod (Int32.v a) (Int32.v b))
+  | S64 -> Int64.int_to_t (Int.sub_mod (Int64.v a) (Int64.v b))
 
 let sub_mod_lemma #t #l a b = ()
 
@@ -208,6 +330,10 @@ let sub #t #l a b =
   | U32  -> UInt32.sub a b
   | U64  -> UInt64.sub a b
   | U128 -> UInt128.sub a b
+  | S8 -> Int8.sub a b
+  | S16 -> Int16.sub a b
+  | S32 -> Int32.sub a b
+  | S64 -> Int64.sub a b
 
 let sub_lemma #t #l a b = ()
 
@@ -219,9 +345,14 @@ let decr #t #l a =
   | U32  -> UInt32.sub a 0x1ul
   | U64  -> UInt64.sub a 0x1uL
   | U128 -> UInt128.sub a (UInt128.uint_to_t 1)
-
+  | S8 -> Int8.sub a 0x1y
+  | S16 -> Int16.sub a 0x1s
+  | S32 -> Int32.sub a 0x1l
+  | S64 -> Int64.sub a 0x1L
+  
 let decr_lemma #t #l a = ()
 
+#reset-options "--z3rlimit 300"
 let logxor #t #l a b =
   match t with
   | U1   ->
@@ -235,26 +366,42 @@ let logxor #t #l a b =
   | U32  -> UInt32.logxor a b
   | U64  -> UInt64.logxor a b
   | U128 -> UInt128.logxor a b
-
+  | S8 -> Int8.logxor a b
+  | S16 -> Int16.logxor a b
+  | S32 -> Int32.logxor a b
+  | S64 -> Int64.logxor a b
+  
 #set-options "--max_fuel 1"
 
 val logxor_lemma_: #t:inttype -> a:uint_t t SEC -> b:uint_t t SEC -> Lemma
   (uint_v (a `logxor` (a `logxor` b)) == uint_v b)
 let logxor_lemma_ #t a b =
+  match t with
+  |U1 |U8 |U16 |U32 |U64 |U128 ->
   UInt.logxor_associative #(bits t) (uint_v a) (uint_v a) (uint_v b);
   UInt.logxor_self #(bits t) (uint_v a);
   UInt.logxor_commutative #(bits t) 0 (uint_v b);
   UInt.logxor_lemma_1 #(bits t) (uint_v b)
+  |S8 |S16 |S32 |S64 ->
+  Int.logxor_associative #(bits t) (uint_v a) (uint_v a) (uint_v b);
+  Int.logxor_self #(bits t) (uint_v a);
+  Int.logxor_commutative #(bits t) 0 (uint_v b);
+  Int.logxor_lemma_1 #(bits t) (uint_v b)
 
 let logxor_lemma #t a b =
   logxor_lemma_ #t a b;
   uintv_extensionality (logxor a (logxor a b)) b;
   assert (a `logxor` (a `logxor` b) == b);
-  UInt.logxor_commutative #(bits t) (uint_v a) (uint_v b);
+  (match t with |U1 |U8 |U16 |U32 |U64 |U128 ->
+   UInt.logxor_commutative #(bits t) (uint_v a) (uint_v b)
+   |S8 |S16 |S32 |S64 -> Int.logxor_commutative #(bits t) (uint_v a) (uint_v b));
   logxor_lemma_ #t a b;
   uintv_extensionality (logxor a (logxor b a)) b;
   assert ((a `logxor` (b `logxor` a)) == b);
-  UInt.logxor_lemma_1 #(bits t) (uint_v a);
+  (match t with |U1 |U8 |U16 |U32 |U64 |U128 ->
+   UInt.logxor_lemma_1 #(bits t) (uint_v a)
+   |S8 |S16 |S32 |S64 -> Int.logxor_lemma_1 #(bits t) (uint_v a));
+  //UInt.logxor_lemma_1 #(bits t) (uint_v a);
   uintv_extensionality (logxor a (uint #t #SEC 0)) a
 
 let logxor_lemma1 #t a b =
@@ -283,14 +430,27 @@ let logand #t #l a b =
   | U32  -> UInt32.logand a b
   | U64  -> UInt64.logand a b
   | U128 -> UInt128.logand a b
+  | S8 -> Int8.logand a b
+  | S16 -> Int16.logand a b
+  | S32 -> Int32.logand a b
+  | S64 -> Int64.logand a b
+
 
 let logand_lemma #t a b =
-  if (uint_v a = 0) then begin
+  match t with |U1 |U8 |U16 |U32 |U64 |U128 ->
+   if (uint_v a = 0) then begin
     UInt.logand_commutative #(bits t) (uint_v a) (uint_v b);
     UInt.logand_lemma_1 #(bits t) (uint_v b) end
   else begin
     UInt.logand_commutative #(bits t) (uint_v a) (uint_v b);
     UInt.logand_lemma_2 #(bits t) (uint_v b) end
+  |S8 |S16 |S32 |S64 ->
+   if (uint_v a = 0) then begin
+    Int.logand_commutative #(bits t) (uint_v a) (uint_v b);
+    Int.logand_lemma_1 #(bits t) (uint_v b) end
+  else begin
+    Int.logand_commutative #(bits t) (uint_v a) (uint_v b);
+    Int.logand_lemma_2 #(bits t) (uint_v b) end
 
 let logand_spec #t #l a b = ()
 
@@ -307,6 +467,10 @@ let logor #t #l a b =
   | U32  -> UInt32.logor a b
   | U64  -> UInt64.logor a b
   | U128 -> UInt128.logor a b
+  | S8 -> Int8.logor a b
+  | S16 -> Int16.logor a b
+  | S32 -> Int32.logor a b
+  | S64 -> Int64.logor a b
 
 let logor_spec #t #l a b = ()
 
@@ -320,7 +484,7 @@ let logor_disjoint #t a b m =
     UInt.logor_commutative #(bits t) (uint_v a) (uint_v b);
     UInt.logor_lemma_1 #(bits t) (uint_v b)
   end
-
+    
 #set-options "--max_fuel 0"
 
 let lognot #t #l a =
@@ -331,7 +495,18 @@ let lognot #t #l a =
   | U32  -> UInt32.lognot a
   | U64  -> UInt64.lognot a
   | U128 -> UInt128.lognot a
+  | S8 -> Int8.lognot a
+  | S16 -> Int16.lognot a
+  | S32 -> Int32.lognot a
+  | S64 -> Int64.lognot a
 
+let shift_right_negative (#n:pos) (a:Int.int_t n{a < 0}) (s:nat) : Tot (Int.int_t n) =
+  let shift_right_negative_vec (#n:pos) (a:BitVector.bv_t n) (s:nat) : Tot (BitVector.bv_t n) =
+  if s>= n then BitVector.ones_vec #n
+  else if s = 0 then a
+  else Seq.append (BitVector.ones_vec #s) (Seq.slice a 0 (n-s))
+  in FStar.Int.from_vec (shift_right_negative_vec #n (FStar.Int.to_vec #n a) s)
+  
 let shift_right #t #l a b =
   match t with
   | U1   -> UInt8.shift_right a b
@@ -340,8 +515,108 @@ let shift_right #t #l a b =
   | U32  -> UInt32.shift_right a b
   | U64  -> UInt64.shift_right a b
   | U128 -> UInt128.shift_right a b
+  | S8 -> Int8.shift_arithmetic_right a b
+  | S16 -> Int16.shift_arithmetic_right a b
+  | S32 -> Int32.shift_arithmetic_right a b
+  | S64 -> Int64.shift_arithmetic_right a b
 
-let shift_right_lemma #t #l a b = ()
+
+#reset-options "--z3rlimit 500 --max_fuel 2 --max_ifuel 2"
+
+val shift_right_value_aux_1: #n:pos{n>1} -> a:Int.int_t n -> s:nat{s >= n} ->
+  Lemma (requires True)
+        (ensures Int.shift_arithmetic_right #n a s = a / pow2 s)
+let shift_right_value_aux_1 #n a s =
+  pow2_le_compat s n;
+  if (a>=0) then (Int.sign_bit_positive a; assert(a=Int.to_uint a); assert(Int.shift_arithmetic_right #n a s == UInt.shift_right #n a s); UInt.shift_right_value_aux_1 #n a s)
+  else begin
+  Int.sign_bit_negative a;
+  assert (Int.shift_arithmetic_right #n a s = -1);
+  assert (- pow2 s <= a /\ a < 0);
+  small_division_lemma_1 (a+pow2 s) (pow2 s);
+  lemma_div_plus a 1 (pow2 s);
+  assert((a+pow2 s) / pow2 s = 0)
+  end
+  
+val shift_right_value_aux_2: #n:pos -> a:Int.int_t n ->
+  Lemma (requires True)
+        (ensures Int.shift_arithmetic_right #n a 0 = a / pow2 0)
+let shift_right_value_aux_2 #n a = assert_norm (pow2 0 == 1)
+
+#reset-options "--z3rlimit 500 --max_fuel 2 --max_ifuel 2"
+
+val append_lemma: #n:pos -> #m:pos -> a:BitVector.bv_t n -> b:BitVector.bv_t m ->
+  Lemma (Int.from_vec #(n + m) (Seq.append a b) = (Int.from_vec #n a) * pow2 m + (UInt.from_vec #m b))
+let append_lemma #n #m a b =
+  let a1 = Int.from_vec #n a in
+  let a2 = UInt.from_vec #n a in
+  let b' = UInt.from_vec #m b in
+  let s1 = Int.from_vec #(n+m) (Seq.append a b) in
+  let s2 = UInt.from_vec #(n+m) (Seq.append a b) in
+  admit()
+
+val shift_right_value_aux_0: #n:pos{n > 1} -> a:Int.int_t n ->
+  Lemma (requires True)
+        (ensures Int.shift_arithmetic_right #n a 1 = a / 2)
+
+let shift_right_value_aux_0 #n a =
+  if a >= 0 then begin
+  Int.sign_bit_positive a; 
+  assert(a=Int.to_uint a); 
+  assert(Int.shift_arithmetic_right #n a 1 == UInt.shift_right #n a 1); 
+  UInt.shift_right_value_aux_3 #n a 1
+  end
+  else begin
+  Int.sign_bit_negative a;
+  let a1 = Int.to_vec a in
+  let au = Int.to_uint a in
+  let sar = Int.shift_arithmetic_right #n a 1 in
+  let sar1 = Int.to_vec sar in
+  let sr = UInt.shift_right #n au 1 in
+  let sr1 = UInt.to_vec sr in
+  assert(Seq.equal (Seq.slice sar1 1 n) (Seq.slice sr1 1 n));
+  assert (Seq.equal sar1 (Seq.append (BitVector.ones_vec #1) (Seq.slice sr1 1 n)));
+  UInt.append_lemma #1 #(n-1) (BitVector.ones_vec #1) (Seq.slice sr1 1 n);
+  assert(Seq.equal (Seq.slice a1 0 (n-1)) (Seq.slice sar1 1 n));
+  UInt.slice_left_lemma a1 (n-1);
+  assert (sar + pow2 n = pow2 (n-1) + (au / 2)); 
+  pow2_double_sum (n-1);
+  assert (sar + pow2 (n-1) = (a + pow2 n) / 2);
+  pow2_double_mult (n-1);
+  lemma_div_plus a (pow2 (n-1)) 2;
+  assert (sar = a / 2)
+  end
+
+
+#reset-options "--z3rlimit 500 --max_fuel 2 --max_ifuel 2"
+
+val shift_right_value_aux_3: #n:pos -> a:Int.int_t n -> s:pos{s < n} ->
+  Lemma (requires True)
+        (ensures Int.shift_arithmetic_right #n a s = a / pow2 s)
+        (decreases s)
+        
+let rec shift_right_value_aux_3 #n a s =
+  if s = 1 then shift_right_value_aux_0 #n a
+  else begin
+  let a1 = Int.to_vec a in
+  assert(Seq.equal (BitVector.shift_arithmetic_right_vec #n a1 s) (BitVector.shift_arithmetic_right_vec #n (BitVector.shift_arithmetic_right_vec #n a1 (s-1)) 1));
+  assert (Int.shift_arithmetic_right #n a s = Int.shift_arithmetic_right #n (Int.shift_arithmetic_right #n a (s-1)) 1);
+  shift_right_value_aux_3 #n a (s-1);
+  shift_right_value_aux_0 #n (Int.shift_arithmetic_right #n a (s-1));
+  assert(Int.shift_arithmetic_right #n a s = (a / pow2 (s-1)) / 2);
+  pow2_double_mult (s-1);
+  division_multiplication_lemma a (pow2 (s-1)) 2
+  end
+
+let shift_right_lemma #t #l a b = 
+  match t with
+  |U1 |U8 |U16 |U32 |U64 |U128 -> ()
+  |_ -> if (uint_v b >= bits t) then shift_right_value_aux_1 #(bits t) (uint_v a) (uint_v b)
+       else if (uint_v b = 0) then shift_right_value_aux_2 #(bits t) (uint_v a)
+       else shift_right_value_aux_3 #(bits t) (uint_v a) (uint_v b)
+  
+let shift_left_negative (#n:pos) (a:Int.int_t n{a < 0}) (s:nat) : Tot (Int.int_t n) =
+  FStar.Int.from_vec (BitVector.shift_left_vec #n (FStar.Int.to_vec #n a) s)
 
 let shift_left #t #l a b =
   match t with
@@ -351,8 +626,39 @@ let shift_left #t #l a b =
   | U32  -> UInt32.shift_left a b
   | U64  -> UInt64.shift_left a b
   | U128 -> UInt128.shift_left a b
+  | S8 -> if (uint_v a >= 0) then Int8.shift_left a b
+         else Int8.int_to_t (shift_left_negative (Int8.v a) (UInt32.v b))
+  | S16 -> if (uint_v a >= 0) then Int16.shift_left a b
+         else Int16.int_to_t (shift_left_negative (Int16.v a) (UInt32.v b))
+  | S32 -> if (uint_v a >= 0) then Int32.shift_left a b
+         else Int32.int_to_t (shift_left_negative (Int32.v a) (UInt32.v b))
+  | S64 -> if (uint_v a >= 0) then Int64.shift_left a b
+         else Int64.int_to_t (shift_left_negative (Int64.v a) (UInt32.v b))
 
-let shift_left_lemma #t #l a b = ()
+#reset-options "--z3rlimit 800 --max_fuel 3 --max_ifuel 3"
+
+let shift_left_lemma #t #l a b = 
+  match t with
+  |U1 |U8 |U16 |U32 |U64 |U128 -> ()
+  |_ -> let a' = uint_v a in
+       let b' = uint_v b in
+       let n = Int.to_uint a' in
+       let sn = UInt.shift_left #(bits t) n b' in
+       assert(Int.to_vec a' == UInt.to_vec #(bits t) n); 
+       if (a' >= 0) then
+       (assert(a' == n);
+       assert (sn == (n * pow2 b') % pow2 (bits t));
+       ()) else
+       (assert(a'+ pow2 (bits t) == n);
+       assert (sn == (n * pow2 b') % pow2 (bits t));
+       assert (sn == ((a'+pow2 (bits t)) * pow2 b') % pow2 (bits t));
+       distributivity_add_left a' (pow2 (bits t)) (pow2 b');
+       assert (sn == ((a'*pow2 b')+(pow2 (bits t)* pow2 b')) % pow2 (bits t));   
+       swap_mul (pow2 (bits t)) (pow2 b');
+       lemma_mod_plus (a' * pow2 b') (pow2 b') (pow2 (bits t));
+       assert (sn == (a' * pow2 b') % pow2 (bits t));
+       ())
+
 
 let rotate_right #t #l a b =
   logor (shift_right a b) (shift_left a (sub #U32 (size (bits t)) b))
@@ -374,7 +680,11 @@ let ones t l =
     let y = (UInt128.shift_left x 64ul) `UInt128.add` x in
     assert_norm (UInt128.v y == pow2 128 - 1);
     y
+  | _  -> uint #t #l (ones_v t)
 
+inline_for_extraction
+let minus (#t:inttype) (#l:secrecy_level) (a:uint_t t l) = add_mod (lognot a) (uint #t #l 1)
+ 
 let eq_mask #t a b =
   match t with
   | U1   -> lognot (logxor a b)
@@ -383,6 +693,12 @@ let eq_mask #t a b =
   | U32  -> UInt32.eq_mask a b
   | U64  -> UInt64.eq_mask a b
   | U128 -> UInt128.eq_mask a b
+  | S8   -> to_i8 #U8 #SEC (UInt8.eq_mask (to_u8 a) (to_u8 b))
+  | S16  -> to_i16 (UInt16.eq_mask (to_u16 a) (to_u16 b))
+  | S32  -> to_i32 (UInt32.eq_mask (to_u32 a) (to_u32 b))
+  | S64  -> to_i64 (UInt64.eq_mask (to_u64 a) (to_u64 b))
+
+#reset-options "--z3rlimit 3000 --max_fuel 1 --max_ifuel 1"
 
 let eq_mask_lemma #t a b =
   match t with
@@ -393,13 +709,62 @@ let eq_mask_lemma #t a b =
       logxor (u1 0) (u1 1) == u1 1 /\ logxor (u1 1) (u1 0) == u1 1 /\
       lognot (u1 1) == u1 0 /\ lognot (u1 0) == u1 1)
     end
-  | _ -> ()
+  | U8 | U16 | U32 | U64 | U128 -> ()
+  | S8 -> let a' = to_u8 a in let b' = to_u8 b in
+  assert_norm (v a = v b <==> v a' = v b');
+    let m' = UInt8.eq_mask a' b' in
+    assert_norm(v #U8 #SEC m' = 0 ==> v #S8 #SEC (to_i8 m') = 0);
+    assert_norm(v #U8 #SEC m' = ones_v U8 ==> v #S8 #SEC (to_i8 #U8 #SEC m') = -1)
+  | S16 -> let a' = to_u16 a in let b' = to_u16 b in
+    assert (v a = v a' @% pow2 16); assert( v a' = v a % pow2 16);
+    assert (v b = v b' @% pow2 16); assert( v b' = v b % pow2 16);
+    let m' = UInt16.eq_mask a' b' in
+    assert (v a' = v b' ==> v m' = ones_v U16);
+    assert (v a' <> v b' ==> v m' = 0);
+    if (v a = v b) then begin
+      assert (v a' = v b');
+      assert (v m' = ones_v U16);
+      assert (v (to_i16 m') = -1) end
+    else begin
+      assert(v a' <> v b');
+      assert(v m' = 0);
+      assert(v (to_i16 m') = 0) end
+  | S32 -> let a' = to_u32 a in let b' = to_u32 b in
+    assert (v a = v a' @% pow2 32); assert( v a' = v a % pow2 32);
+    assert (v b = v b' @% pow2 32); assert( v b' = v b % pow2 32);
+    let m' = UInt32.eq_mask a' b' in
+    assert (v a' = v b' ==> v m' = ones_v U32);
+    assert (v a' <> v b' ==> v m' = 0);
+    if (v a = v b) then begin
+      assert (v a' = v b');
+      assert (v m' = ones_v U32);
+      assert (v (to_i32 m') = -1) end
+    else begin
+      assert(v a' <> v b');
+      assert(v m' = 0);
+      assert(v (to_i32 m') = 0) end
+  | S64 -> let a' = to_u64 a in let b' = to_u64 b in
+    assert (v a = v a' @% pow2 64); assert( v a' = v a % pow2 64);
+    assert (v b = v b' @% pow2 64); assert( v b' = v b % pow2 64);
+    let m' = UInt64.eq_mask a' b' in
+    assert (v a' = v b' ==> v m' = ones_v U64);
+    assert (v a' <> v b' ==> v m' = 0);
+    if (v a = v b) then begin
+      assert (v a' = v b');
+      assert (v m' = ones_v U64);
+      assert (v (to_i64 m') = -1) end
+    else begin
+      assert(v a' <> v b');
+      assert(v m' = 0);
+      assert(v (to_i64 m') = 0) end
 
 let eq_mask_logand_lemma #t a b c =
   eq_mask_lemma a b;
   logand_lemma (eq_mask a b) c;
-  UInt.logand_commutative #(bits t) (uint_v (eq_mask a b)) (uint_v c)
-
+  match t with 
+  | U8 | U16 | U32 | U64 | U128 -> UInt.logand_commutative #(bits t) (uint_v (eq_mask a b)) (uint_v c)
+  | _ -> Int.logand_commutative #(bits t) (uint_v (eq_mask a b)) (uint_v c)
+  
 let neq_mask #t a b = lognot (eq_mask #t a b)
 
 let gte_mask #t a b =
@@ -433,8 +798,9 @@ let gt_mask #t a b = logand (gte_mask a b) (neq_mask a b)
 
 let lte_mask #t a b = logor (lt_mask a b) (eq_mask a b)
 
+#reset-options "--z3rlimit 3000 --max_fuel 3 --max_ifuel 3"
 private
-val mod_mask_value: #t:inttype -> #l:secrecy_level -> m:shiftval t ->
+val mod_mask_value: #t:inttype{~(S8? t) /\ ~(S16? t) /\ ~(S32? t) /\ ~(S64? t)} -> #l:secrecy_level -> m:shiftval t ->
   Lemma (uint_v (mod_mask #t #l m) == pow2 (uint_v m) - 1)
 let mod_mask_value #t #l m =
   if uint_v m > 0 then begin
@@ -467,7 +833,7 @@ let div #t x y =
   | U16 -> UInt16.div x y
   | U32 -> UInt32.div x y
   | U64 -> UInt64.div x y
-
+  
 let div_lemma #t x y = ()
 
 let mod #t x y =
@@ -488,7 +854,11 @@ let eq #t x y =
   | U32 -> UInt32.eq x y
   | U64 -> UInt64.eq x y
   | U128 -> UInt128.eq x y
-
+  | S8  -> Int8.eq x y
+  | S16 -> Int16.eq x y
+  | S32 -> Int32.eq x y
+  | S64 -> Int64.eq x y
+  
 let eq_lemma #t x y = ()
 
 let ne #t x y =
@@ -499,7 +869,11 @@ let ne #t x y =
   | U32 -> not (UInt32.eq x y)
   | U64 -> not (UInt64.eq x y)
   | U128 -> not (UInt128.eq x y)
-
+  | S8  -> not (Int8.eq x y)
+  | S16 -> not (Int16.eq x y)
+  | S32 -> not (Int32.eq x y)
+  | S64 -> not (Int64.eq x y)
+  
 let ne_lemma #t x y = ()
 
 let lt #t x y =
@@ -510,7 +884,11 @@ let lt #t x y =
   | U32 -> UInt32.lt x y
   | U64 -> UInt64.lt x y
   | U128 -> UInt128.lt x y
-
+  | S8  -> Int8.lt x y
+  | S16 -> Int16.lt x y
+  | S32 -> Int32.lt x y
+  | S64 -> Int64.lt x y
+  
 let lt_lemma #t x y = ()
 
 let lte #t x y =
@@ -521,7 +899,11 @@ let lte #t x y =
   | U32 -> UInt32.lte x y
   | U64 -> UInt64.lte x y
   | U128 -> UInt128.lte x y
-
+  | S8  -> Int8.lte x y
+  | S16 -> Int16.lte x y
+  | S32 -> Int32.lte x y
+  | S64 -> Int64.lte x y
+  
 let lte_lemma #t x y = ()
 
 let gt #t x y =
@@ -532,7 +914,11 @@ let gt #t x y =
   | U32 -> UInt32.gt x y
   | U64 -> UInt64.gt x y
   | U128 -> UInt128.gt x y
-
+  | S8  -> Int8.gt x y
+  | S16 -> Int16.gt x y
+  | S32 -> Int32.gt x y
+  | S64 -> Int64.gt x y
+  
 let gt_lemma #t x y = ()
 
 let gte #t x y =
@@ -543,5 +929,9 @@ let gte #t x y =
   | U32 -> UInt32.gte x y
   | U64 -> UInt64.gte x y
   | U128 -> UInt128.gte x y
-
+  | S8  -> Int8.gte x y
+  | S16 -> Int16.gte x y
+  | S32 -> Int32.gte x y
+  | S64 -> Int64.gte x y
+  
 let gte_lemma #t x y = ()
