lib/Lib.IntTypes.fsti
@@ -8,8 +8,7 @@ open FStar.Math.Lemmas
 ///
 
 type inttype =
-  | U1 | U8 | U16 | U32 | U64 | U128
-
+  | U1 | U8 | U16 | U32 | U64 | U128 | S8 | S16 | S32 | S64
 ///
 /// Operations on the underlying machine integer base types
 ///
@@ -19,20 +18,39 @@ let bits (n:inttype) =
   match n with
   | U1 -> 1
   | U8 -> 8
+  | S8 -> 8
   | U16 -> 16
+  | S16 -> 16
   | U32 -> 32
+  | S32 -> 32
   | U64 -> 64
+  | S64 -> 64
   | U128 -> 128
+  //| S128 -> 128
+
+inline_for_extraction
+let range (x:int) (n:inttype) : Type0 =
+  match n with
+  | U1 | U8 | U16 | U32 | U64 | U128 -> UInt.size x (bits n)
+  | S8 | S16 | S32 | S64 -> Int.size x (bits n)
+
+inline_for_extraction
+type range_t (n:inttype) = x:int{range x n}
 
 inline_for_extraction
 let numbytes (n:inttype) =
   match n with
   | U1 -> 1
   | U8 -> 1
+  | S8 -> 1
   | U16 -> 2
+  | S16 -> 2
   | U32 -> 4
+  | S32 -> 4
   | U64 -> 8
+  | S64 -> 8
   | U128 -> 16
+  //| S128 -> 16
 
 val pow2_values: n:nat ->  Lemma (
     pow2 0 == 1 /\
@@ -53,8 +71,16 @@ unfold let modulus (t:inttype) = pow2 (bits t)
 
 inline_for_extraction
 unfold let maxint (t:inttype) =
-  modulus t - 1
-
+  match t with
+  | U1 | U8 | U16 | U32 | U64 | U128 -> UInt.max_int (bits t)
+  | S8 | S16 | S32 | S64 -> Int.max_int (bits t)
+  
+inline_for_extraction
+unfold let minint (t:inttype) =
+  match t with
+  | U1 | U8 | U16 | U32 | U64 | U128 -> UInt.min_int (bits t)
+  | S8 | S16 | S32 | S64 -> Int.min_int (bits t)
+  
 (* PUBLIC Machine Integers *)
 
 inline_for_extraction
@@ -66,9 +92,14 @@ let pub_int_t (t:inttype) =
   | U32 -> UInt32.t
   | U64 -> UInt64.t
   | U128 -> UInt128.t
+  | S8 -> Int8.t
+  | S16 -> Int16.t
+  | S32 -> Int32.t
+  | S64 -> Int64.t
+  //| S128 -> Int128.t
 
 inline_for_extraction
-let pub_int_v #t (x:pub_int_t t) : (n:nat{n <= maxint t}) =
+let pub_int_v #t (x:pub_int_t t) : (n:range_t t) =
   match t with
   | U1 -> UInt8.v x
   | U8 -> UInt8.v x
@@ -76,6 +107,11 @@ let pub_int_v #t (x:pub_int_t t) : (n:nat{n <= maxint t}) =
   | U32 -> UInt32.v x
   | U64 -> UInt64.v x
   | U128 -> UInt128.v x
+  | S8 -> Int8.v x
+  | S16 -> Int16.v x
+  | S32 -> Int32.v x
+  | S64 -> Int64.v x
+  //| S128 -> Int128.v x
 
 (* SECRET Machine Integers *)
 
@@ -87,7 +123,7 @@ inline_for_extraction
 val sec_int_t: t:inttype -> Type0
 
 inline_for_extraction
-val sec_int_v: #t:inttype -> u:sec_int_t t -> n:nat{n <= maxint t}
+val sec_int_v: #t:inttype -> u:sec_int_t t -> n:range_t t
 
 (* GENERIC (unsigned) Machine Integers *)
 
@@ -97,7 +133,7 @@ let uint_t (t:inttype) (l:secrecy_level) =
   | PUB -> pub_int_t t
   | SEC -> sec_int_t t
 
-let uint_v #t #l (u:uint_t t l) : n:nat{n <= maxint t} =
+let uint_v #t #l (u:uint_t t l) : n:range_t t =
   match l with
   | PUB -> pub_int_v #t u
   | SEC -> sec_int_v #t u
@@ -122,16 +158,31 @@ inline_for_extraction
 type uint8 = uint_t U8 SEC
 
 inline_for_extraction
+type int8 = uint_t S8 SEC
+
+inline_for_extraction
 type uint16 = uint_t U16 SEC
+
+inline_for_extraction
+type int16 = uint_t S16 SEC
 
 inline_for_extraction
 type uint32 = uint_t U32 SEC
 
 inline_for_extraction
+type int32 = uint_t S32 SEC
+
+inline_for_extraction
 type uint64 = uint_t U64 SEC
 
 inline_for_extraction
+type int64 = uint_t S64 SEC
+
+inline_for_extraction
 type uint128 = uint_t U128 SEC
+
+//inline_for_extraction
+//type int128 = uint_t S128 SEC
 
 inline_for_extraction
 unfold type bit_t = uint_t U1 PUB
@@ -143,17 +194,31 @@ inline_for_extraction
 unfold type size_t = uint_t U32 PUB
 
 inline_for_extraction
+unfold type pub_int8 = uint_t S8 PUB
+
+inline_for_extraction
 unfold type pub_uint16 = uint_t U16 PUB
+
+inline_for_extraction
+unfold type pub_int16 = uint_t S16 PUB
 
 inline_for_extraction
 unfold type pub_uint32 = uint_t U32 PUB
 
 inline_for_extraction
+unfold type pub_int32 = uint_t S32 PUB
+
+inline_for_extraction
 unfold type pub_uint64 = uint_t U64 PUB
+
+inline_for_extraction
+unfold type pub_int64 = uint_t S64 PUB
 
 inline_for_extraction
 unfold type pub_uint128 = uint_t U128 PUB
 
+//inline_for_extraction
+//unfold type pub_int128 = uint_t S128 PUB
 ///
 /// Casts between natural numbers and machine integers
 ///
@@ -162,7 +227,7 @@ inline_for_extraction
 val secret: #t:inttype -> u:uint_t t PUB -> v:uint_t t SEC{uint_v v == uint_v u}
 
 inline_for_extraction
-val uint: #t:inttype -> #l:secrecy_level -> (n:nat{n <= maxint t}) -> u:uint_t t l{uint_v u == n}
+val uint: #t:inttype -> #l:secrecy_level -> (n:range_t t) -> u:uint_t t l{uint_v u == n}
 
 val uintv_injective:
    #t:inttype
@@ -172,23 +237,38 @@ val uintv_injective:
  [SMTPat (uint_v #t #l a)]
 
 inline_for_extraction
-let u1 (n:nat{n <= maxint U1}) : u:uint1{uint_v #U1 u == n} = uint #U1 #SEC n
+let u1 (n:range_t U1) : u:uint1{uint_v #U1 u == n} = uint #U1 #SEC n
 
 inline_for_extraction
-let u8 (n:nat{n <= maxint U8}) : u:uint8{uint_v #U8 u == n} = uint #U8 #SEC n
+let u8 (n:range_t U8) : u:uint8{uint_v #U8 u == n} = uint #U8 #SEC n
 
 inline_for_extraction
-let u16 (n:nat{n <= maxint U16}) : u:uint16{uint_v #U16 u == n} = uint #U16 #SEC n
+let i8 (n:range_t S8) : u:int8{uint_v #S8 u == n} = uint #S8 #SEC n
 
 inline_for_extraction
-let u32 (n:nat{n <= maxint U32}) : u:uint32{uint_v #U32 u == n} = uint #U32 #SEC n
+let u16 (n:range_t U16) : u:uint16{uint_v #U16 u == n} = uint #U16 #SEC n
 
 inline_for_extraction
-let u64 (n:nat{n <= maxint U64}) : u:uint64{uint_v #U64 u == n} = uint #U64 #SEC n
+let i16 (n:range_t S16) : u:int16{uint_v #S16 u == n} = uint #S16 #SEC n
+
+inline_for_extraction
+let u32 (n:range_t U32) : u:uint32{uint_v #U32 u == n} = uint #U32 #SEC n
+
+inline_for_extraction
+let i32 (n:range_t S32) : u:int32{uint_v #S32 u == n} = uint #S32 #SEC n
+
+inline_for_extraction
+let u64 (n:range_t U64) : u:uint64{uint_v #U64 u == n} = uint #U64 #SEC n
+
+inline_for_extraction
+let i64 (n:range_t S64) : u:int64{uint_v #S64 u == n} = uint #S64 #SEC n
 
 (* We only support 64-bit literals, hence the unexpected upper limit in the following function *)
 inline_for_extraction
-val u128: n:nat{n <= maxint U64} -> u:uint128{uint_v #U128 u == n}
+val u128: (n:range_t U64) -> u:uint128{uint_v #U128 u == n}
+
+//inline_for_extraction
+//let i128 (n:range_t S128) : u:int128{uint_v #S128 u == n} = uint #S128 #SEC n
 
 unfold noextract
 let max_size_t = maxint U32
@@ -233,28 +313,58 @@ val size_to_uint64: s:size_t -> u:uint64{u == u64 (uint_v s)}
 inline_for_extraction
 val byte_to_uint8: s:byte_t -> u:uint8{u == u8 (byte_v s)}
 
+let op_At_Percent = Int.op_At_Percent
+
+#reset-options
 inline_for_extraction
-val nat_to_uint: #t:inttype -> #l:secrecy_level -> (n:nat{n <= maxint t}) -> u:uint_t t l{uint_v u == n}
+val byte_to_int8: s:byte_t -> u:int8{u == i8 ((byte_v s) @% 256)}
+
+inline_for_extraction
+val nat_to_uint: #t:inttype -> #l:secrecy_level -> (n:range_t t) -> u:uint_t t l{uint_v u == n}
+
+inline_for_extraction
+let op_At_Percent_Dot x t =
+  match t with
+  | U1 | U8 | U16 | U32 | U64 | U128 -> x % modulus t
+  | S8 | S16 | S32 | S64 -> x @% modulus t
 
 inline_for_extraction
 val cast: #t:inttype -> #l:secrecy_level
-          -> t':inttype -> l':secrecy_level {PUB? l \/ SEC? l'}
-          -> u1:uint_t t l -> u2:uint_t t' l'{uint_v u2 == uint_v u1 % modulus t'}
+          -> t':inttype{(~(U128? t')) \/ (U1? t) \/ (U8? t) \/ (U16? t) \/ (U32? t) \/ (U64? t) \/ (U128? t)} -> l':secrecy_level {PUB? l \/ SEC? l'}
+          -> u1:uint_t t l -> u2:uint_t t' l'{uint_v u2 == uint_v u1 @%. t'}
+
+inline_for_extraction
+let to_u1 #t #l u : uint1 = cast #t #l U1 SEC u
 
 inline_for_extraction
 let to_u8 #t #l u : uint8 = cast #t #l U8 SEC u
 
 inline_for_extraction
+let to_i8 #t #l u : int8 = cast #t #l S8 SEC u
+
+inline_for_extraction
 let to_u16 #t #l u : uint16 = cast #t #l U16 SEC u
+
+inline_for_extraction
+let to_i16 #t #l u : int16 = cast #t #l S16 SEC u
 
 inline_for_extraction
 let to_u32 #t #l u : uint32 = cast #t #l U32 SEC u
 
 inline_for_extraction
+let to_i32 #t #l u : int32 = cast #t #l S32 SEC u
+
+inline_for_extraction
 let to_u64 #t #l u : uint64 = cast #t #l U64 SEC u
 
 inline_for_extraction
-let to_u128 #t #l u : uint128 = cast #t #l U128 SEC u
+let to_i64 #t #l u : int64 = cast #t #l S64 SEC u
+
+inline_for_extraction
+let to_u128 (#t:inttype{(U1? t) \/ (U8? t) \/ (U16? t) \/ (U32? t) \/ (U64? t) \/ (U128? t)}) #l u : uint128 = cast #t #l U128 SEC u
+
+//inline_for_extraction
+//let to_i128 #t #l u : int128 = cast #t #l S128 SEC u
 
 ///
 /// Bitwise operators for all machine integers
@@ -271,19 +381,19 @@ val add_mod_lemma: #t:inttype -> #l:secrecy_level ->
              a:uint_t t l ->
              b:uint_t t l ->
 	     Lemma
-	     (ensures (uint_v #t #l (add_mod #t #l a b) == (uint_v a + uint_v b) % modulus t))
+	     (ensures (uint_v #t #l (add_mod #t #l a b) == (uint_v a + uint_v b) @%. t))
 	     [SMTPat (uint_v #t #l (add_mod #t #l a b))]
 
 inline_for_extraction
 val add: #t:inttype -> #l:secrecy_level
   -> a:uint_t t l
-  -> b:uint_t t l{uint_v a + uint_v b < modulus t}
+  -> b:uint_t t l{range (uint_v a + uint_v b) t}
   -> uint_t t l
 
 inline_for_extraction
 val add_lemma: #t:inttype -> #l:secrecy_level
   -> a:uint_t t l
-  -> b:uint_t t l{uint_v a + uint_v b < modulus t}
+  -> b:uint_t t l{range (uint_v a + uint_v b) t}
   -> Lemma
     (ensures (uint_v #t #l (add #t #l a b) == uint_v a + uint_v b))
     [SMTPat (uint_v #t #l (add #t #l a b))]
@@ -310,20 +420,20 @@ val mul_mod_lemma: #t:inttype{t <> U128} -> #l:secrecy_level
   -> a:uint_t t l
   -> b:uint_t t l
   -> Lemma
-  (ensures (uint_v #t #l (mul_mod #t #l a b) == (uint_v a `op_Multiply` uint_v b) % modulus t))
+  (ensures (uint_v #t #l (mul_mod #t #l a b) == (uint_v a `op_Multiply` uint_v b) @%. t))
   [SMTPat (uint_v #t #l (mul_mod #t #l a b))]
 
 inline_for_extraction
 val mul: #t:inttype{t <> U128} -> #l:secrecy_level
   -> a:uint_t t l
-  -> b:uint_t t l{uint_v a `op_Multiply` uint_v b < modulus t}
+  -> b:uint_t t l{range (uint_v a `op_Multiply` uint_v b) t}
   -> uint_t t l
 
 
 inline_for_extraction
 val mul_lemma: #t:inttype{t <> U128} -> #l:secrecy_level
   -> a:uint_t t l
-  -> b:uint_t t l{uint_v a `op_Multiply` uint_v b < modulus t}
+  -> b:uint_t t l{range (uint_v a `op_Multiply` uint_v b) t}
   -> Lemma
   (ensures (uint_v #t #l (mul #t #l a b) == uint_v a `op_Multiply` uint_v b))
   [SMTPat (uint_v #t #l (mul #t #l a b))]
@@ -338,6 +448,14 @@ val mul64_wide_lemma: a:uint64 -> b:uint64
   (ensures (uint_v (mul64_wide a b) == uint_v a `op_Multiply` uint_v b))
   [SMTPat (uint_v (mul64_wide a b))]
 
+//inline_for_extraction
+//val mulsigned64_wide: a:int64 -> b:int64 -> int128
+
+//inline_for_extraction
+//val mulsigned64_wide_lemma: a:int64 -> b:int64
+  //-> Lemma
+  //(ensures (uint_v (mulsigned64_wide a b) == uint_v a `op_Multiply` uint_v b))
+  //[SMTPat (uint_v (mulsigned64_wide a b))]
 (* KB: I would prefer the post-condition to say:
        uint_v c = (pow2 (bits t) + uint_v a - uint_v b) % pow2 (bits t)
 *)
@@ -352,33 +470,47 @@ val sub_mod_lemma: #t:inttype -> #l:secrecy_level ->
              a:uint_t t l ->
              b:uint_t t l ->
 	     Lemma
-	     (ensures (uint_v #t #l (sub_mod #t #l a b) == (uint_v a - uint_v b) % modulus t))
+	     (ensures (uint_v #t #l (sub_mod #t #l a b) == (uint_v a - uint_v b) @%. t))
 	     [SMTPat (uint_v #t #l (sub_mod #t #l a b))]
 
 inline_for_extraction
 val sub: #t:inttype -> #l:secrecy_level
   -> a:uint_t t l
-  -> b:uint_t t l{uint_v a >= uint_v b}
+  -> b:uint_t t l{range (uint_v a - uint_v b) t}
   -> uint_t t l
 
 inline_for_extraction
 val sub_lemma: #t:inttype -> #l:secrecy_level ->
              a:uint_t t l ->
-             b:uint_t t l{uint_v a >= uint_v b} ->
+             b:uint_t t l{range (uint_v a - uint_v b) t} ->
 	     Lemma
 	     (ensures (uint_v #t #l (sub #t #l a b) == uint_v a - uint_v b))
 	     [SMTPat (uint_v #t #l (sub #t #l a b))]
 
 inline_for_extraction
 val decr: #t:inttype -> #l:secrecy_level
-  -> a:uint_t t l{uint_v a > 0}
+  -> a:uint_t t l{uint_v a > minint t}
   -> uint_t t l
 
 inline_for_extraction
 val decr_lemma: #t:inttype -> #l:secrecy_level
-  -> a:uint_t t l{uint_v a > 0}
+  -> a:uint_t t l{uint_v a > minint t}
   -> Lemma
   (ensures (uint_v #t #l (decr a) == uint_v a - 1))
+
+inline_for_extraction
+let zero (t:inttype) = 0
+
+inline_for_extraction
+let one (t:inttype) = 1
+
+#reset-options
+inline_for_extraction
+let ones_v (t:inttype) =
+  match t with
+  | U1 | U8 | U16 | U32 | U64 | U128 -> maxint t
+  | S8 | S16 | S32 | S64 -> -1
+
 
 inline_for_extraction
 val logxor: #t:inttype -> #l:secrecy_level
@@ -392,8 +524,8 @@ val logxor_lemma: #t:inttype -> a:uint_t t SEC -> b:uint_t t SEC -> Lemma
    a `logxor` (uint #t #SEC 0) == a)
 
 val logxor_lemma1: #t:inttype -> a:uint_t t SEC -> b:uint_t t SEC -> Lemma
-  (requires v a <= 1 /\ v b <= 1)
-  (ensures v (a `logxor` b) <= 1)
+  (requires range (v a) U1 /\ range (v b) U1)
+  (ensures range (v (a `logxor` b)) U1)
 
 inline_for_extraction
 val logand: #t:inttype -> #l:secrecy_level
@@ -402,12 +534,17 @@ val logand: #t:inttype -> #l:secrecy_level
   -> uint_t t l
 
 val logand_lemma: #t:inttype{~(U1? t)} -> a:uint_t t SEC -> b:uint_t t SEC -> Lemma
-  (requires v a = 0 \/ v a = maxint t)
-  (ensures (if v a = 0 then v (a `logand` b) == 0 else v (a `logand` b) == v b))
+  (requires v a = zero t \/ v a = ones_v t)
+  (ensures (if v a = zero t then v (a `logand` b) == zero t else v (a `logand` b) == v b))
 
+let logand_v (#t:inttype{~(U1? t)}) (a: range_t t) (b:range_t t) : range_t t=
+match t with
+  |S8 | S16 | S32 | S64 -> Int.logand #(8*numbytes t) a b
+  |_ -> UInt.logand #(8*numbytes t) a b
+  
 val logand_spec: #t:inttype{~(U1? t)} -> #l:secrecy_level
   -> a:uint_t t l -> b:uint_t t l
-  -> Lemma (ensures (v (a `logand` b) == v a `UInt.logand #(8 * numbytes t)` v b))
+  -> Lemma (ensures (v (a `logand` b) == (v a `logand_v` v b)))
   //[SMTPat (v (a `logand` b))]
 
 inline_for_extraction
@@ -416,8 +553,8 @@ val logor: #t:inttype -> #l:secrecy_level
   -> b:uint_t t l
   -> uint_t t l
 
-val logor_disjoint: #t:inttype -> a:uint_t t SEC -> b:uint_t t SEC -> m:nat{m < bits t} -> Lemma
-  (requires v a < pow2 m /\ v b % pow2 m == 0)
+val logor_disjoint: #t:inttype{(U1? t) \/ (U8? t) \/ (U16? t) \/ (U32? t) \/ (U64? t) \/ (U128? t)} -> a:uint_t t SEC -> b:uint_t t SEC -> m:nat{m < bits t} -> Lemma
+  (requires 0 <= v a /\ v a < pow2 m /\ v b % pow2 m == 0)
   (ensures v (a `logor` b) == v a + v b)
 
 inline_for_extraction
@@ -441,7 +578,7 @@ val shift_right_lemma: #t:inttype -> #l:secrecy_level
   -> a:uint_t t l
   -> b:shiftval t
   -> Lemma
-    (uint_v #t #l (shift_right #t #l a b) ==  uint_v #t #l a / pow2 (uint_v #U32 #PUB b))
+    (ensures uint_v #t #l (shift_right #t #l a b) ==  uint_v #t #l a / pow2 (uint_v #U32 #PUB b))
     [SMTPat (uint_v #t #l (shift_right #t #l a b))]
 
 inline_for_extraction
@@ -454,7 +591,7 @@ val shift_left_lemma: #t:inttype -> #l:secrecy_level
   -> a:uint_t t l
   -> b:shiftval t
   -> Lemma
-    (uint_v #t #l (shift_left #t #l a b) == (uint_v #t #l a `op_Multiply` pow2 (uint_v #U32 #PUB b)) % modulus t)
+    (uint_v #t #l (shift_left #t #l a b) == (uint_v #t #l a `op_Multiply` pow2 (uint_v #U32 #PUB b)) @%. t)
     [SMTPat (uint_v #t #l (shift_left #t #l a b))]
 
 inline_for_extraction
@@ -474,54 +611,54 @@ val rotate_left: #t:inttype -> #l:secrecy_level
 ///
 
 inline_for_extraction
-val zeroes: t:inttype -> l:secrecy_level -> v:uint_t t l{uint_v v = 0}
+val zeroes: t:inttype -> l:secrecy_level -> v:uint_t t l{uint_v v = zero t}
 
 inline_for_extraction
-val ones: t:inttype -> l:secrecy_level -> v:uint_t t l{uint_v v = maxint t}
+val ones: t:inttype -> l:secrecy_level -> v:uint_t t l{uint_v v = ones_v t}
 
 inline_for_extraction
-val eq_mask: #t:inttype -> uint_t t SEC -> uint_t t SEC -> uint_t t SEC
+val eq_mask: #t:inttype{~(S64? t)} -> uint_t t SEC -> uint_t t SEC -> uint_t t SEC
 
-val eq_mask_lemma: #t:inttype -> a:uint_t t SEC -> b:uint_t t SEC -> Lemma
+val eq_mask_lemma: #t:inttype{~(S64? t)} -> a:uint_t t SEC -> b:uint_t t SEC -> Lemma
   (requires True)
-  (ensures  (v a = v b ==> v (eq_mask a b) == maxint t) /\
+  (ensures  (v a = v b ==> v (eq_mask a b) == ones_v t) /\
             (v a <> v b ==> v (eq_mask a b) == 0))
   [SMTPat (eq_mask #t a b)]
 
-val eq_mask_logand_lemma: #t:inttype{~(U1? t)} -> a:uint_t t SEC -> b:uint_t t SEC -> c:uint_t t SEC -> Lemma
+val eq_mask_logand_lemma: #t:inttype{~(U1? t) /\ ~(S64? t)} -> a:uint_t t SEC -> b:uint_t t SEC -> c:uint_t t SEC -> Lemma
   (ensures (if v a = v b then v (c `logand` (eq_mask a b)) == v c else v (c `logand` (eq_mask a b)) == 0))
   [SMTPat (c `logand` (eq_mask a b))]
 
 inline_for_extraction
-val neq_mask: #t:inttype -> a:uint_t t SEC -> b:uint_t t SEC -> uint_t t SEC
+val neq_mask: #t:inttype{~(S64? t)} -> a:uint_t t SEC -> b:uint_t t SEC -> uint_t t SEC
 
 inline_for_extraction
-val gte_mask: #t:inttype -> uint_t t SEC -> b:uint_t t SEC -> uint_t t SEC
+val gte_mask: #t:inttype{~(S8? t) /\ ~(S16? t) /\ ~(S32? t) /\ ~(S64? t)} -> uint_t t SEC -> b:uint_t t SEC -> uint_t t SEC
 
-val gte_mask_lemma: #t:inttype -> a:uint_t t SEC -> b:uint_t t SEC -> Lemma
+val gte_mask_lemma: #t:inttype{~(S8? t) /\ ~(S16? t) /\ ~(S32? t) /\ ~(S64? t)} -> a:uint_t t SEC -> b:uint_t t SEC -> Lemma
   (requires True)
   (ensures  (v a >= v b ==> v (gte_mask a b) == maxint t) /\
             (v a < v b ==> v (gte_mask a b) == 0))
   [SMTPat (gte_mask #t a b)]
 
-val gte_mask_logand_lemma: #t:inttype{~(U1? t)} -> a:uint_t t SEC -> b:uint_t t SEC -> c:uint_t t SEC -> Lemma
+val gte_mask_logand_lemma: #t:inttype{~(U1? t) /\ ~(S8? t) /\ ~(S16? t) /\ ~(S32? t) /\ ~(S64? t)} -> a:uint_t t SEC -> b:uint_t t SEC -> c:uint_t t SEC -> Lemma
   (ensures (if v a >= v b then v (c `logand` (gte_mask a b)) == v c else v (c `logand` (gte_mask a b)) == 0))
   [SMTPat (c `logand` (gte_mask a b))]
 
 inline_for_extraction
-val lt_mask: #t:inttype -> uint_t t SEC -> uint_t t SEC -> uint_t t SEC
+val lt_mask: #t:inttype{~(S8? t) /\ ~(S16? t) /\ ~(S32? t) /\ ~(S64? t)} -> uint_t t SEC -> uint_t t SEC -> uint_t t SEC
 
 inline_for_extraction
-val gt_mask: #t:inttype -> uint_t t SEC -> b:uint_t t SEC -> uint_t t SEC
+val gt_mask: #t:inttype{~(S8? t) /\ ~(S16? t) /\ ~(S32? t) /\ ~(S64? t)} -> uint_t t SEC -> b:uint_t t SEC -> uint_t t SEC
 
 inline_for_extraction
-val lte_mask: #t:inttype -> uint_t t SEC -> uint_t t SEC -> uint_t t SEC
+val lte_mask: #t:inttype{~(S8? t) /\ ~(S16? t) /\ ~(S32? t) /\ ~(S64? t)} -> uint_t t SEC -> uint_t t SEC -> uint_t t SEC
 
 inline_for_extraction
-let mod_mask (#t:inttype) (#l:secrecy_level) (m:shiftval t) : uint_t t l =
+let mod_mask (#t:inttype{~(S8? t) /\ ~(S16? t) /\ ~(S32? t) /\ ~(S64? t)}) (#l:secrecy_level) (m:shiftval t) : uint_t t l =
   (nat_to_uint 1 `shift_left` m) `sub_mod` nat_to_uint 1
 
-val mod_mask_lemma: #t:inttype -> #l:secrecy_level -> a:uint_t t l -> m:shiftval t ->
+val mod_mask_lemma: #t:inttype{~(S8? t) /\ ~(S16? t) /\ ~(S32? t) /\ ~(S64? t)} -> #l:secrecy_level -> a:uint_t t l -> m:shiftval t ->
   Lemma
     (requires True)
     (ensures  uint_v (a `logand` (mod_mask #t m)) == uint_v a % pow2 (uint_v m))
@@ -578,13 +715,13 @@ let ( ~. ) #t #l = lognot #t #l
 ///
 
 inline_for_extraction
-val div: #t:inttype{t <> U128}
+val div: #t:inttype{t <> U128 /\ ~(S8? t) /\ ~(S16? t) /\ ~(S32? t) /\ ~(S64? t)}
   -> a:uint_t t PUB
   -> b:uint_t t PUB{uint_v b > 0}
   -> uint_t t PUB
 
 inline_for_extraction
-val div_lemma: #t:inttype{t <> U128}
+val div_lemma: #t:inttype{t <> U128 /\ ~(S8? t) /\ ~(S16? t) /\ ~(S32? t) /\ ~(S64? t)}
   -> a:uint_t t PUB
   -> b:uint_t t PUB{uint_v b > 0}
   -> Lemma
@@ -593,10 +730,10 @@ val div_lemma: #t:inttype{t <> U128}
 
 
 inline_for_extraction
-val mod: #t:inttype{t <> U128} -> a:uint_t t PUB -> b:uint_t t PUB{uint_v b > 0} -> uint_t t PUB
+val mod: #t:inttype{t <> U128 /\ ~(S8? t) /\ ~(S16? t) /\ ~(S32? t) /\ ~(S64? t)} -> a:uint_t t PUB -> b:uint_t t PUB{uint_v b > 0} -> uint_t t PUB
 
 inline_for_extraction
-val mod_lemma: #t:inttype{t <> U128}
+val mod_lemma: #t:inttype{t <> U128 /\ ~(S8? t) /\ ~(S16? t) /\ ~(S32? t) /\ ~(S64? t)}
   -> a:uint_t t PUB
   -> b:uint_t t PUB{uint_v b > 0}
   -> Lemma
